define encode_len and impl for all primitive types

proof/defs.v
@@ -1,11 +1,19 @@
-From Minirust.def Require Import ty encoding utils thm.
+From Minirust.def Require Import ty encoding utils thm wf.
 
 Definition canonicalize ty l := decode ty l >>= encode ty.
+
+Definition encode_len (ty: Ty) :=
+  wf ty ->
+  forall v, forall l,
+  is_valid_for ty v ->
+  encode ty v = Some l ->
+  length l = ty_size ty.
 
 (* will be extended by helper properties satisfied by all well-formed types *)
 Record Props ty := {
   PR_RT1 : rt1 ty;
   PR_RT2 : rt2 ty;
   PR_MONO1 : mono1 ty;
-  PR_MONO2 : mono2 ty
+  PR_MONO2 : mono2 ty;
+  PR_ENCODE_LEN : encode_len ty
 }.
